Proof of equivalence of infinite traces

src/Trace.v
@@ -126,6 +126,163 @@ Fixpoint to_of_run {E A} {x : C.t E A} {v_x : A} (r_x : Run.t x v_x)
     now rewrite H1; rewrite H2.
 Qed.
 
+Module I.
+  Module Trace.
+    CoInductive t (E : Effect.t) : Type :=
+    | Ret : t E
+    | Call : forall c, Effect.answer E c -> t E
+    | Let : t E -> t E -> t E
+    | ChooseLeft : t E -> t E
+    | ChooseRight : t E -> t E
+    | Join : t E -> t E -> t E.
+    Arguments Ret {E}.
+    Arguments Call {E} _ _.
+    Arguments Let {E} _ _.
+    Arguments ChooseLeft {E} _.
+    Arguments ChooseRight {E} _.
+    Arguments Join {E} _ _.
+
+    Definition unfold {E} (t : Trace.t E) : Trace.t E :=
+      match t with
+      | Ret => Ret
+      | Call c a => Call c a
+      | Let t_x t_f => Let t_x t_f
+      | ChooseLeft t => ChooseLeft t
+      | ChooseRight t => ChooseRight t
+      | Join t_x t_y => Join t_x t_y
+      end.
+
+    Lemma unfold_eq {E} (t : Trace.t E) : t = unfold t.
+      destruct t; reflexivity.
+    Defined.
+
+    Module Eq.
+      CoInductive t {E} : Trace.t E -> Trace.t E -> Prop :=
+      | Ret : t Ret Ret
+      | Call : forall c a, t (Call c a) (Call c a)
+      | Let : forall t_x1 t_x2 t_f1 t_f2, t t_x1 t_x2 -> t t_f1 t_f2 ->
+        t (Let t_x1 t_f1) (Let t_x2 t_f2)
+      | ChooseLeft : forall t1 t2, t t1 t2 ->
+        t (ChooseLeft t1) (ChooseLeft t2)
+      | ChooseRight : forall t1 t2, t t1 t2 ->
+        t (ChooseRight t1) (ChooseRight t2)
+      | Join : forall t_x1 t_x2 t_y1 t_y2, t t_x1 t_x2 -> t t_y1 t_y2 ->
+        t (Join t_x1 t_y1) (Join t_x2 t_y2).
+    End Eq.
+  End Trace.
+
+  Module Valid.
+    CoInductive t {E} : forall {A}, C.I.t E A -> Trace.t E -> A -> Type :=
+    | Ret : forall A (v : A), t (C.I.Ret A v) Trace.Ret v
+    | Call : forall c (a : Effect.answer E c), t (C.I.Call c) (Trace.Call c a) a
+    | Let : forall A B (x : C.I.t E A) (f : A -> C.I.t E B)
+      (t_x t_y : Trace.t E) (v_x : A) (v_y : B),
+      t x t_x v_x -> t (f v_x) t_y v_y ->
+      t (C.I.Let _ _ x f) (Trace.Let t_x t_y) v_y
+    | ChooseLeft : forall A (x1 x2 : C.I.t E A) (t_x1 : Trace.t E) (v_x1 : A),
+      t x1 t_x1 v_x1 -> t (C.I.Choose _ x1 x2) (Trace.ChooseLeft t_x1) v_x1
+    | ChooseRight : forall A (x1 x2 : C.I.t E A) (t_x2 : Trace.t E) (v_x2 : A),
+      t x2 t_x2 v_x2 -> t (C.I.Choose _ x1 x2) (Trace.ChooseRight t_x2) v_x2
+    | Join : forall A B (x : C.I.t E A) (y : C.I.t E B) (t_x t_y : Trace.t E)
+      (v_x : A) (v_y : B),
+      t x t_x v_x -> t y t_y v_y ->
+      t (C.I.Join _ _ x y) (Trace.Join t_x t_y) (v_x, v_y).
+    Arguments Ret {E A} _.
+    Arguments Call {E} _ _.
+    Arguments Let {E A B x f t_x t_y v_x v_y} _ _.
+    Arguments ChooseLeft {E A x1 x2 t_x1 v_x1} _.
+    Arguments ChooseRight {E A x1 x2 t_x2 v_x2} _.
+    Arguments Join {E A B x y t_x t_y v_x v_y} _ _.
+
+    Definition unfold {E A} {x : C.I.t E A} {t : Trace.t E} {v : A}
+      (H : Valid.t x t v) : Valid.t x t v :=
+      match H with
+      | Ret _ v => Ret v
+      | Call c a => Call c a
+      | Let _ _ _ _ _ _ _ _ H_x H_f => Let H_x H_f
+      | ChooseLeft _ _ _ _ _ H_x1 => ChooseLeft H_x1
+      | ChooseRight _ _ _ _ _ H_x2 => ChooseRight H_x2
+      | Join _ _ _ _ _ _ _ _ H_x H_y => Join H_x H_y
+      end.
+
+    Lemma unfold_eq {E A} {x : C.I.t E A} {t : Trace.t E} {v : A}
+      (H : Valid.t x t v) : H = unfold H.
+      destruct H; reflexivity.
+    Qed.
+  End Valid.
+
+  CoFixpoint trace_of_run {E A} {x : C.I.t E A} {v_x : A} (r_x : Run.I.t x v_x)
+    : Trace.t E.
+    destruct r_x.
+    - exact Trace.Ret.
+    - exact (Trace.Call c answer).
+    - exact (Trace.Let (trace_of_run _ _ _ _ r_x1) (trace_of_run _ _ _ _ r_x2)).
+    - exact (Trace.ChooseLeft (trace_of_run _ _ _ _ r_x)).
+    - exact (Trace.ChooseRight (trace_of_run _ _ _ _ r_x)).
+    - exact (Trace.Join
+        (trace_of_run _ _ _ _ r_x1) (trace_of_run _ _ _ _ r_x2)).
+  Defined.
+
+  CoFixpoint valid_of_run {E A} {x : C.I.t E A} {v_x : A} (r_x : Run.I.t x v_x)
+    : Valid.t x (trace_of_run r_x) v_x.
+    rewrite (Trace.unfold_eq (trace_of_run _)).
+    destruct r_x; simpl.
+    - apply Valid.Ret.
+    - apply Valid.Call.
+    - eapply Valid.Let; apply valid_of_run.
+    - apply Valid.ChooseLeft; apply valid_of_run.
+    - apply Valid.ChooseRight; apply valid_of_run.
+    - apply Valid.Join; apply valid_of_run.
+  Defined.
+
+  CoFixpoint to_run {E A} {x : C.I.t E A} {t_x : Trace.t E} {v_x : A}
+    (H : Valid.t x t_x v_x) : Run.I.t x v_x.
+    destruct H.
+    - apply Run.I.Ret.
+    - apply Run.I.Call.
+    - eapply Run.I.Let.
+      + eapply to_run.
+        apply H.
+      + eapply to_run.
+        apply H0.
+    - apply Run.I.ChooseLeft.
+      eapply to_run.
+      apply H.
+    - apply Run.I.ChooseRight.
+      eapply to_run.
+      apply H.
+    - apply Run.I.Join.
+      + eapply to_run.
+        apply H.
+      + eapply to_run.
+        apply H0.
+  Defined.
+
+  CoFixpoint trace_of_to_run {E A} {x : C.I.t E A} {t_x : Trace.t E} {v_x : A}
+    (H : Valid.t x t_x v_x) : Trace.Eq.t (trace_of_run (to_run H)) t_x.
+    rewrite (Trace.unfold_eq (trace_of_run _)).
+    destruct H; simpl.
+    - apply Trace.Eq.Ret.
+    - apply Trace.Eq.Call.
+    - apply Trace.Eq.Let; apply trace_of_to_run.
+    - apply Trace.Eq.ChooseLeft; apply trace_of_to_run.
+    - apply Trace.Eq.ChooseRight; apply trace_of_to_run.
+    - apply Trace.Eq.Join; apply trace_of_to_run.
+  Qed.
+
+  CoFixpoint to_of_run {E A} {x : C.I.t E A} {v : A} (r : Run.I.t x v)
+    : Run.I.Eq.t (to_run (valid_of_run r)) r.
+    rewrite (Run.I.unfold_eq (to_run _)).
+    destruct r; simpl.
+    - apply Run.I.Eq.Ret.
+    - apply Run.I.Eq.Call.
+    - apply Run.I.Eq.Let; apply to_of_run.
+    - apply Run.I.Eq.ChooseLeft; apply to_of_run.
+    - apply Run.I.Eq.ChooseRight; apply to_of_run.
+    - apply Run.I.Eq.Join; apply to_of_run.
+  Qed.
+End I.
+
 Module Test.
   Require Import Coq.Lists.List.
   Require Import Coq.Strings.Ascii.
@@ -192,12 +349,12 @@ Module Test.
     end.
 
   Definition get_name_uc (name : LString.t) : Run.t get_name (Some name).
-    eapply Let. apply (Run.Call (E := E) (Command.Print _) tt).
+    eapply Run.Let. apply (Run.Call (E := E) (Command.Print _) tt).
     apply (Run.Call (E := E) Command.ReadLine (Some name)).
   Defined.
 
   Definition your_name2_uc (name : LString.t) : Run.t your_name2 tt.
-    eapply Let. apply (get_name_uc name).
+    eapply Run.Let. apply (get_name_uc name).
     apply (Run.Call (E := E) (Command.Print (LString.s _ ++ name)) tt).
   Defined.
 End Test.
